Kura/Planarity/Plainarity.lean
@@ -16,15 +16,14 @@ variable {V E F : Type*} [LinearOrder V] [LinearOrder E] [LinearOrder F] (G : Gr
 --     edgeEmbedding e 1 = vertexEmbedding (G.ends e).snd)
 
 structure AbstractDual (H : Graph F E) where
-  cycle_minEdgeCut (w : Cycle G) : H.minEdgeCut w.edges.toFinset
-  minEdgeCut_cycle (S : Finset E) : G.minEdgeCut S → ∃ (w : Cycle H),
-    S = w.edges.toFinset
+  minEdgeCut_cycle (S : Set E) : G.minEdgeCut S ↔ ∃ (w : Cycle H), S = w.edges.toFinset
 
 class Planar_by_AbstractDual :=
   F : Type*
   FLinearOrder : LinearOrder F
   FNonempty : Nonempty F
   dualGraph : Graph F E
+  dualGraphUndir : dualGraph.Undirected
   dualGraphConn : dualGraph.connected
   isDual : AbstractDual G dualGraph
 
@@ -37,6 +36,10 @@ instance instPlanar_by_AbstractDualFLinearOrder :
 instance instPlanar_by_AbstractDualFacesLinearOrder :
     LinearOrder G.Faces := Planar_by_AbstractDual.FLinearOrder
 def dualGraph := Planar_by_AbstractDual.dualGraph (G := G)
+instance instPlanar_by_AbstractDualdualGraphUndirected :
+    Undirected G.dualGraph := Planar_by_AbstractDual.dualGraphUndir
+instance instPlanar_by_AbstractDualdualGraphConnected :
+    connected G.dualGraph := Planar_by_AbstractDual.dualGraphConn
 def duality : AbstractDual G (dualGraph G) := Planar_by_AbstractDual.isDual
 
 
@@ -49,14 +52,20 @@ instance instPlanar_by_AbstractDualFacesFintype [Fintype E]:
 
 lemma bridge_iff_loop [Planar_by_AbstractDual G] :
     G.bridge e ↔ G.dualGraph.isLoop e := by
-
   constructor <;> rintro h
   · have hmincut := G.bridge_is_minEdgeCut e h
-    have  := G.duality.minEdgeCut_cycle {e} sorry
+    have  := (G.duality.minEdgeCut_cycle {e}).mp hmincut
     obtain ⟨W, hW⟩ := this
-    sorry
+    have : W.edges = [e] := sorry
+    exact W.isLoop_of_edges_singleton G.dualGraph e this
+  · let v := (G.dualGraph.get e).inf
+    obtain C : G.dualGraph.Cycle := Cycle.ofLoop G.dualGraph e h
 
-  · sorry
+    have hmincut := (G.duality.minEdgeCut_cycle C.edges.toFinset).mpr ⟨C, rfl⟩
+    have : C.edges.toFinset = {e} := sorry
+    simp only [this, Finset.coe_singleton] at hmincut
+    exact edgeCut_of_minEdgeCut G {e} hmincut
+
 
 instance doubleDual [Fintype V] [Nonempty V] [Planar_by_AbstractDual G] [G.nConnected 3] :
     Planar_by_AbstractDual (dualGraph G) where
@@ -64,6 +73,7 @@ instance doubleDual [Fintype V] [Nonempty V] [Planar_by_AbstractDual G] [G.nConn
   FLinearOrder := by assumption
   FNonempty := by assumption
   dualGraph := G
+  dualGraphUndir := by assumption
   dualGraphConn := G.connected_of_nConnected 3
   isDual := sorry
 
@@ -86,7 +96,7 @@ theorem EulerFormula [Nonempty V] [Fintype V] [Fintype E] [G.connected]:
     have h0lt: Fintype.card V > 0 := Fintype.card_pos
     have : Fintype.card V = 1 := Eq.symm (Nat.le_antisymm h0lt hle1)
     rw [this]; clear h hle1 h0lt this
-    
+
     sorry
 
 
